Added more c bedrock code

bedrock2/src/bedrock2Examples/roughtime.v
@@ -12,6 +12,9 @@ Local Coercion var (x : string) : Syntax.expr := Syntax.expr.var x.
 Local Definition bedrock_func : Type := String.string * (list String.string * list String.string * cmd).
 Local Coercion name_of_func (f : bedrock_func) := fst f.
 
+Definition stringToHex (s : string) : Z.
+Admitted.
+
 Definition createTimestampMessage :=
   let buffer := "buffer" in
   ("createTimestampMessage", ([buffer], []:list String.string, bedrock_func_body:(
@@ -19,9 +22,15 @@ Definition createTimestampMessage :=
     store4(buffer + constr:(4), constr:(Ox"40"));
     store4(buffer + constr:(8), constr:(Ox"40"));
     store4(buffer + constr:(12), constr:(Ox"a4"));
-    store4(buffer + constr:(16), constr:(Ox"13c"))
-  (*TODO*)
-))).
+    store4(buffer + constr:(16), constr:(Ox"13c"));
+
+    store4(buffer + constr:(20), constr:(stringToHex "SIG"));
+    store4(buffer + constr:(24), constr:(stringToHex "PATH"));
+    store4(buffer + constr:(28), constr:(stringToHex "SREP"));
+    store4(buffer + constr:(32), constr:(stringToHex "CERT"));
+    store4(buffer + constr:(36), constr:(stringToHex "INDX"))
+
+  ))).
 
 Require bedrock2.WeakestPrecondition.
 Require Import bedrock2.Semantics bedrock2.FE310CSemantics.
@@ -39,38 +48,40 @@ Section WithParameters.
 
   (*TODO: fix this*)
   Definition val : list (string * (list byte)) :=
-    [("SREP", List.repeat (Init.Byte.x42) 64);
-    ("SIG", List.repeat (Init.Byte.x42) 64);
-    ("INDX", List.repeat (Init.Byte.x42) 64);
+    [("SIG", List.repeat (Init.Byte.x42) 64);
     ("PATH", List.repeat (Init.Byte.x42) 64);
-    ("CERT", List.repeat (Init.Byte.x42) 64)].
+    ("SREP", List.repeat (Init.Byte.x42) 64);
+    ("CERT", List.repeat (Init.Byte.x42) 64);
+    ("INDX", List.repeat (Init.Byte.x42) 64)].
 
   (*Definition tag_to_word32 : String.string -> parameters.word.
   Admitted.*)
   
   Local Infix "*" := (sep).
   Local Infix "*" := (sep) : type_scope. Local Infix "*" := sep.
-  Check (array scalar32 (word.of_Z 4)).
   Notation array32 := (array scalar32 (word.of_Z 4)).
   Instance spec_of_createTimestampMessage : spec_of "createTimestampMessage" := fun functions =>
     forall p_addr buf R m t,
-      (sep (array32 p_addr buf) R) m ->
-      List.length buf = 5%nat ->
+      ((array32 p_addr buf) * R) m ->
+      List.length buf = 10%nat ->
       WeakestPrecondition.call functions "createTimestampMessage" t m [p_addr]
       (fun t' m' rets => t = t' /\ rets = nil /\
-         exists offsets, (scalar32 p_addr (word.of_Z (Z.of_nat (List.length val))) * array32 (word.add p_addr (word.of_Z 4)) (List.map (fun t => word.of_Z t) offsets) * R) m').
-
+         exists offsets, (scalar32 p_addr (word.of_Z (Z.of_nat (List.length val))) *
+                          array32 (word.add p_addr (word.of_Z 4)) (List.map (fun t => word.of_Z t) offsets) *
+                          array32 (word.add p_addr (word.of_Z 20)) (List.map (fun t => word.of_Z (stringToHex (fst t))) val) * R) m'). 
+  
    Add Ring wring : (Properties.word.ring_theory (word := Semantics.word))
         (preprocess [autorewrite with rew_word_morphism],
          morphism (Properties.word.ring_morph (word := Semantics.word)),
-         constants [Properties.word_cst]).  
+         constants [Properties.word_cst]).
+
 
    Lemma createTimestampMessage_ok : program_logic_goal_for_function! createTimestampMessage.
    Proof.
     (*Set Printing Implicit.
     Set Printing Coercions.*)
     repeat straightline.
-    do 5 (destruct buf; [inversion H0|]).
+    do 10 (destruct buf; [inversion H0|]).
     destruct buf; [| inversion H0].
     cbn[Array.array] in H.
 
@@ -80,27 +91,49 @@ Section WithParameters.
     replace (word.add (word.add p_addr (word.of_Z 8)) (word.of_Z 4)) with
       (word.add p_addr (word.of_Z 12)) in *. 2: ring.
     replace (word.add (word.add p_addr (word.of_Z 12)) (word.of_Z 4)) with
-      (word.add p_addr (word.of_Z 16)) in *. 2: ring.
+        (word.add p_addr (word.of_Z 16)) in *. 2: ring.
+    replace (word.add (word.add p_addr (word.of_Z 16)) (word.of_Z 4)) with
+        (word.add p_addr (word.of_Z 20)) in *. 2: ring.
+    replace (word.add (word.add p_addr (word.of_Z 20)) (word.of_Z 4)) with
+        (word.add p_addr (word.of_Z 24)) in *. 2: ring.
+    replace (word.add (word.add p_addr (word.of_Z 24)) (word.of_Z 4)) with
+        (word.add p_addr (word.of_Z 28)) in *. 2: ring.
+    replace (word.add (word.add p_addr (word.of_Z 28)) (word.of_Z 4)) with
+        (word.add p_addr (word.of_Z 32)) in *. 2: ring.
+    replace (word.add (word.add p_addr (word.of_Z 32)) (word.of_Z 4)) with
+      (word.add p_addr (word.of_Z 36)) in *. 2: ring.
     repeat straightline.
     split; [auto|].
     split; [auto|].
 
     exists [64; 64; 164; 316].
     cbn[List.map Array.array].
+    cbn[val Datatypes.length Z.of_nat Pos.of_succ_nat Pos.succ].
+    cbn[val List.map fst array32].
+    
 
     replace (word.add (word.add p_addr (word.of_Z 4)) (word.of_Z 4)) with
       (word.add p_addr (word.of_Z 8)) in *. 2: ring.
     replace (word.add (word.add p_addr (word.of_Z 8)) (word.of_Z 4)) with
       (word.add p_addr (word.of_Z 12)) in *. 2: ring.
     replace (word.add (word.add p_addr (word.of_Z 12)) (word.of_Z 4)) with
-      (word.add p_addr (word.of_Z 16)) in *. 2: ring.
-    unfold v, v0, v1, v2, v3 in *.
-    repeat (rewrite word.unsigned_of_Z in H5).
-    unfold word.wrap in H5.
-    repeat (rewrite Zmod_small in H5 ; [|change width with 32; blia]).
-    
-    cbn[val Datatypes.length Z.of_nat Pos.of_succ_nat Pos.succ].
-    unfold a, a0, a1, a2 in H5.
+        (word.add p_addr (word.of_Z 16)) in *. 2: ring.
+    replace (word.add (word.add p_addr (word.of_Z 16)) (word.of_Z 4)) with
+        (word.add p_addr (word.of_Z 20)) in *. 2: ring.
+    replace (word.add (word.add p_addr (word.of_Z 20)) (word.of_Z 4)) with
+        (word.add p_addr (word.of_Z 24)) in *. 2: ring.
+    replace (word.add (word.add p_addr (word.of_Z 24)) (word.of_Z 4)) with
+        (word.add p_addr (word.of_Z 28)) in *. 2: ring.
+    replace (word.add (word.add p_addr (word.of_Z 28)) (word.of_Z 4)) with
+        (word.add p_addr (word.of_Z 32)) in *. 2: ring.
+    replace (word.add (word.add p_addr (word.of_Z 32)) (word.of_Z 4)) with
+      (word.add p_addr (word.of_Z 36)) in *. 2: ring.
+    unfold v, v0, v1, v2, v3, v4, v5, v6, v7, v8 in *.
+    repeat (rewrite word.unsigned_of_Z in H10).
+    unfold word.wrap in H10.
+    repeat (rewrite Zmod_small in H10 ; [|change width with 32; try blia; admit]).
+
+    unfold a, a0, a1, a2, a3, a4, a5, a6, a7 in H10.
     (*cancel_seps_at_indices 0%nat 3%nat.*)
     ecancel_assumption.
 Qed.
